\documentclass{article}
\usepackage{amsmath}
\usepackage{amssymb}
\usepackage{geometry}
\usepackage{bm} 
\newcommand{\R}{\mathbb{R}}
\geometry{a4paper, margin=1in}

\title{MSBD 5007 HW1}
\author{RONG Shuo}
\date{\today}

\begin{document}

\maketitle

\section*{Question1}
Given two vectors \(\bm{a} = [a_0, a_1, \cdots, a_{N - 1}]\) and \(\bm{b} = [b_0, b_1, \cdots, b_{N-1}]^T\), their \textit{circular convolution} is defined by
\[(\bm{a} \circledast\bm{b})_k = \sum_{j = 0}^{N - 1} a_j b_{k - j}, k = 0, 1, \cdots, N - 1,\]
where \(\bm{b}\) is extended periodically, i.e., \(b_{k - j} = b_{(k - j) + N}\) if \(-N \leq k-j \leq -1\). Let \(\bm{f}, \bm{g}, \) and \(\bm{h}\) be vectors in \(\R^N\). Prove that the circular convolution satisfies:

(a) \(\bm{f}\circledast  \bm{g} = \bm{g} \circledast \bm{f}\). 

(b) \(\bm{f}\circledast (\bm{g} \circledast \bm{h}) = (\bm{f} \circledast \bm{g}) \circledast \bm{h}\). 
\subsection*{(a)}
\begin{align*}
    (\bm{f} \circledast\bm{g})_k & \\  
    &= \sum_{j = 0}^{N - 1} f_j g_{k - j} \\
    &= \sum_{j = k + 1}^{N - 1} f_j g_{k - j} + \sum_{j = 0}^{k} f_j g_{k - j}  \\
    &= \sum_{j = k + 1}^{N - 1} f_j g_{N + k - j} + \sum_{j = 0}^{k} f_j g_{k - j}  \\
    &= \sum_{i = k + 1}^{N - 1} f_{N + k - i} g_{i} + \sum_{j = 0}^{k} f_j g_{k - j}  \\
    &= \sum_{i = k + 1}^{N - 1}  g_{i} f_{k - i} + \sum_{i = 0}^{k} f_{k - i} g_i  \\
    &= \sum_{i = k + 1}^{N - 1}  g_{i} f_{k - i} + \sum_{i = 0}^{k} g_i f_{k - i}  \\
    &= \sum_{i = 0}^{N - 1} g_{i} f_{k - i} \\
    &= (\bm{g} \circledast \bm{f})_k
\end{align*}
Therefore, we can conclude that: \(\bm{f}\circledast  \bm{g} = \bm{g} \circledast \bm{f}\). 

\subsection*{(b)}
\begin{align*}
    (\bm{f} \circledast (\bm{g} \circledast \bm{h}))_k &= (\bm{f} \circledast (\bm{h} \circledast \bm{g}))_k \\ 
    &= \sum_{j = 0}^{N-1} f_j(\bm{h} \circledast \bm{g})_{k - j} \\
    &= \sum_{j = 0}^{N-1} f_j \sum_{i = 0}^{N-1} h_i g_{k - j - i} \\
    &= \sum_{j = 0}^{N-1}  \sum_{i = 0}^{N-1} f_j h_i g_{k - j - i} \\
    &= \sum_{i = 0}^{N-1} \sum_{j = 0}^{N-1} f_j h_i g_{k - j - i} \\
    &= \sum_{i = 0}^{N-1} h_i \sum_{j = 0}^{N-1} f_j  g_{k - j - i} \\
    &= \sum_{i = 0}^{N-1} h_i(\bm{f} \circledast \bm{g})_{k - j} \\
    &= (\bm{h} \circledast (\bm{f} \circledast \bm{g}))_k \\
    &= ((\bm{f} \circledast \bm{g}) \circledast \bm{h})_k
\end{align*}
Therefore, we can conclude that: \(\bm{f}\circledast (\bm{g} \circledast \bm{h}) = (\bm{f} \circledast \bm{g}) \circledast \bm{h}\). 

\end{document}